hoare_example/ImpIO.v
@@ -1,0 +1,32 @@
+From Coq Require Import
+     Arith.PeanoNat
+     Lists.List
+     Strings.String
+     Morphisms
+     Setoid
+     RelationClasses.
+
+Inductive aexp :=
+  | AId : string -> aexp
+  | ANum : nat -> aexp
+  | APlus : aexp -> aexp -> aexp
+  | AMinus : aexp -> aexp -> aexp
+  | AMult : aexp -> aexp -> aexp
+.
+
+Inductive bexp :=
+  | BEq : aexp -> aexp -> bexp
+  | BLeq : aexp -> aexp -> bexp
+  | BNot : bexp -> bexp
+  | BAnd : bexp -> bexp
+  | BTrue : bexp
+.
+
+Inductive com :=
+  | CSeq : com -> com -> com
+  | CIf : bexp -> com -> com -> com
+  | CAss : string -> aexp -> com
+  | CWhile : bexp -> com -> com
+  | CPrint : aexp -> com
+  | CRead : string -> com
+.
