Makefile
@@ -10,7 +10,7 @@ all:
 	# Build the library before tests
 	$(MAKE) coq
 	$(MAKE) test
-	$(MAKE) tutorial
+	$(MAKE) hoare_example
 
 install: Makefile.coq coq
 	$(MAKE) -f $< $@
@@ -30,11 +30,16 @@ examples:
 tutorial:
 	$(MAKE) -C tutorial
 
+hoare_example:
+	$(MAKE) -C hoare_example
+
+
 clean: clean-coq
 	$(RM) _CoqProject
 	$(MAKE) -C tests clean
 	$(MAKE) -C examples clean
 	$(MAKE) -C tutorial clean
+	$(MAKE) -C hoare_example clean
 
 _CoqProject: $(COQPATHFILE) _CoqConfig Makefile
 	@ echo "# Generating _CoqProject"
